%! Author = Админ
%! Date = 18.02.2022

% Packages
\documentclass[11pt]{article}
\usepackage{amsmath}
\usepackage{graphicx}
\usepackage{mathtools}
\usepackage{gensymb}

\graphicspath{{pictures/}}


% Document
\begin{document}
    \section{Problem}
    a)
    \includegraphics[width=200px]{cube.png}
    \[
        \overline{|BC|}=(c_{1}-b_{1};c_{2}-b_{2};c_{3}-b_{3})=(2;0;2)
    \]
    \[
        l=\overline{|BC|}=\sqrt{x^2 + y^2 + z^2}=2\sqrt{2}
    \]
    BC equals to the diagonal of the square, and since all faces of the cube are equal squares, their diagonals are equal too.\newline
    b)
    The angle between H and C is equal to the angle between the vectors $\overline{OB}$ and $\overline{OC}$:
    \[
        \alpha=\arccos(\frac{\overline{OB}\cdot\overline{OC}}{|\overline{OB}| |\overline{OC}|})=109.47\degree
    \]
    c)
    \[
        \angle (CBD) = \arccos(\frac {\overline{BC}\cdot \overline{BD}}{|\overline{BC}| |\overline{BD}|}) = 60\degree
    \]
    \[
        \angle \beta = \arccos(\frac {\overline{AB}\cdot \overline{DC}}{|\overline{AB}| |\overline{DC}|}) = 90 \degree
    \]
    d)
    \[
        S = \frac{BC^2\cdot\sqrt{3}}{4} = 2\sqrt{3}
    \]


    \section{Problem}
    a)
    \[
        \overline{v_1}\cdot(\overline{v_2}-\overline{v_3})=0
    \]
    b-c)
    \[
        \overline{v_1}\cdot\overline{v_2}=\overline{v_1}\cdot\overline{v_3}=\overline{v_2}\cdot\overline{v_3}
    => \overline{v_1}=\overline{v_2}=\overline{v_3} \] =\textgreater the triangle is equilateral and $P$ is also on the altitude from $P_3$


    \section{Problem}
    \includegraphics[width=200px]{tetr.png}
    \[\overline{a}\times\overline{b}=\overline{v_1} \]
    \[\overline{c}\times\overline{a}=\overline{v_2} \]
    \[\overline{b}\times\overline{c}=\overline{v_3} \]
    \[\overline{v_1}=det(\begin{bmatrix}
                           \overline{i} & \overline{j} & \overline{k}\\
                           a_1 & a_2 & a_3 \\
                           b_1 & b_2 & b_3
    \end{bmatrix}) = \overline{i}\cdot(a_2b_3 - a_3b_2)-\overline{j}\cdot(a_1b_3 - a_3b_1) + \overline{k} \cdot(a_1b_2-a_2b_1) \newline \]
    \[\overline{v_2}=det(\begin{bmatrix}
                           \overline{i} & \overline{j} & \overline{k}\\
                           c_1 & c_2 & c_3 \\
                           a_1 & a_2 & a_3
    \end{bmatrix}) = \overline{i}\cdot(c_2a_3 - c_3a_2)-\overline{j}\cdot(c_1a_3 - c_3a_1) + \overline{k} \cdot(c_1a_2-c_2a_1) \newline \]
    \[\overline{v_3}=det(\begin{bmatrix}
                           \overline{i} & \overline{j} & \overline{k}\\
                           b_1 & b_2 & b_3 \\
                           c_1 & c_2 & c_3
    \end{bmatrix}) = \overline{i}\cdot(b_2c_3 - b_3c_2)-\overline{j}\cdot(b_1c_3 - b_3c_1) + \overline{k} \cdot(b_1c_2-b_2c_1) \newline \]
    \[\overline{v_4}=det(\begin{bmatrix}
                           \overline{i} & \overline{j} & \overline{k}\\
                           (\overline{b}-\overline{c})_1 & (\overline{b}-\overline{c})_2 & (\overline{b}-\overline{c})_3 \\
                           (\overline{a}-\overline{c})_1 & (\overline{a}-\overline{c})_2 & (\overline{a}-\overline{c})_3
    \end{bmatrix}) = \overline{i}\cdot((\overline{b}-\overline{c})_2(\overline{a}-\overline{c})_3 - (\overline{b}-\overline{c})_3(\overline{a}-\overline{c})_2)-\overline{j}\cdot((\overline{b}-\overline{c})_1(\overline{a}-\overline{c})_3 - \newline \]
    \[ -(\overline{b}-\overline{c})_3(\overline{a}-\overline{c})_1) + \overline{k} \cdot((\overline{b}-\overline{c})_1(\overline{a}-\overline{c})_2-(\overline{b}-\overline{c})_2(\overline{a}-\overline{c})_1) = \overline{i}\cdot(b_2a_3-b_2c_3-c_2a_3+c_2c_3-b_3a_2+b_3c_2+c_3a_2- \newline \]
    \[ -c_2c_3)+\overline{j}\cdot(b_1a_3-b_1c_3-c_1a_3+c_1c_3-b_3a_1+b_3c_1+c_3a_1-c_1c_3)+\overline{k}\cdot(b_1a_2-a_2c_1-c_2b_1+c_2c_1-b_2a_1+b_2c_1+ \newline\]
    \( +c_2a_1-c_2c_1)  \)
    \[ \overline{v_1}+\overline{v_2}+\overline{v_3}+\overline{v_4}=\overline{i}\cdot(a_2b_3 - a_3b_2+c_2a_3 - c_3a_2+b_2c_3 - b_3c_2+b_2a_3-b_2c_3-c_2a_3-b_3a_2+b_3c_2+c_3a_2)+ \newline \]
    \[ +\overline{j}\cdot(a_1b_3 - a_3b_1+c_1a_3 - c_3a_1+b_1c_3 - b_3c_1+b_1a_3-b_1c_3-c_1a_3+c_1c_3-b_3a_1+b_3c_1+c_3a_1-c_1c_3)+ \newline \]
    \[ +\overline{k}\cdot(a_1b_2-a_2b_1+c_1a_2-c_2a_1+b_1c_2-b_2c_1+b_1a_2-a_2c_1-c_2b_1+c_2c_1-b_2a_1+b_2c_1+c_2a_1-c_2c_1)=0  \newline\]


    \section{Problem}
    a)
    \includegraphics[width=200px]{coord1.png}
    \[ A=\begin{bmatrix}
            \frac{\sqrt{2}}{2} & -\frac{\sqrt{2}}{2} \\
            \frac{\sqrt{2}}{2} & \frac{\sqrt{2}}{2}
    \end{bmatrix} \]
    \[ \overline{v}=A \begin{bmatrix}
                       0\\
                       1
    \end{bmatrix} = \begin{bmatrix}
                        -0.7\\
                        0.7
    \end{bmatrix} \newline \]
    \[\overline{u}=A \begin{bmatrix}
                       1\\
                       0
    \end{bmatrix} = \begin{bmatrix}
                        0.7\\
                        0.7
    \end{bmatrix} \newline\]
    b)
    \[ \begin{bmatrix}
        \cos(\alpha) & -\sin(\alpha)\\
        \sin(\alpha) & \cos(\alpha)
    \end{bmatrix} \times \begin{bmatrix}
                             \cos(\beta) & -\sin(\beta)\\
                             \sin(\beta) & \cos(\beta)
    \end{bmatrix} = \]
    \[ = \begin{bmatrix}
                        \cos(\alpha)\cdot\cos(\beta)-\sin(\alpha)\cdot\sin(\beta) & -\cos(\alpha)\cdot\sin(\beta)-\sin(\alpha)\cdot\cos(\beta)\\
                        \sin(\alpha)\cdot\sin(\beta)+\cos(\alpha)\cdot\cos(\beta) & \cos(\alpha)\cdot\cos(\beta)-\sin(\alpha)\cdot\sin(\beta)
    \end{bmatrix} = \]
    \[ \begin{bmatrix}
                        \cos(\alpha+\beta) & -\sin(\alpha+\beta)\\
                        \sin(\alpha+\beta) & \cos(\alpha+\beta)
    \end{bmatrix} \]
    c)
    \[ d=det(\begin{bmatrix}
                \cos(\alpha) & -\sin(\alpha)\\
                \sin(\alpha) & \cos(\alpha)
    \end{bmatrix}) = \cos(\alpha)^2+\sin(\alpha)^2=1 \]
    \[ M_*=(\begin{bmatrix}
               \cos(\alpha)  & \sin(\alpha)\\
               -\sin(\alpha) & \cos(\alpha)
    \end{bmatrix}) \]
    \[ A^{-1}=\frac{1}{d}\cdot M_*=M_* \]
    1)
    \[ \begin{bmatrix}
                     \cos(\alpha)  & \sin(\alpha)\\
                     -\sin(\alpha) & \cos(\alpha)
    \end{bmatrix} \times \begin{bmatrix}
                             \cos(\alpha)  & -\sin(\alpha)\\
                             \sin(\alpha) & \cos(\alpha)
    \end{bmatrix} = \begin{bmatrix}
                        1 & 0\\
                        0 & 1
    \end{bmatrix} = I \]
    2)
    \[ \begin{bmatrix}
                     \cos(-\alpha)  & -\sin(-\alpha)\\
                     \sin(-\alpha)  &  \cos(-\alpha)
    \end{bmatrix} = \begin{bmatrix}
                        \cos(\alpha)  & \sin(\alpha)\\
                        -\sin(\alpha) & \cos(\alpha)
    \end{bmatrix} \]
    \[ => A_\theta^{-1}=A_{-\theta} \]

    d) \newline
    1)
    \[\begin{bmatrix}
                     -\frac{\sqrt{2}}{2} & -\frac{\sqrt{2}}{2} \\
                     \frac{\sqrt{2}}{2}  & -\frac{\sqrt{2}}{2}
    \end{bmatrix} \]
    2)
    \[\begin{bmatrix}
                     -\frac{\sqrt{2}}{2} & -\frac{\sqrt{2}}{2} \\
                     -\frac{\sqrt{2}}{2} &  \frac{\sqrt{2}}{2}
    \end{bmatrix} \]
    3)
    \[ \begin{bmatrix}
                     -\frac{\sqrt{2}}{2} &  \frac{\sqrt{2}}{2} \\
                     -\frac{\sqrt{2}}{2} & -\frac{\sqrt{2}}{2}
    \end{bmatrix} \]
    4)
    \[\begin{bmatrix}
                     -\frac{\sqrt{2}}{2} & \frac{\sqrt{2}}{2} \\
                     \frac{\sqrt{2}}{2}  & \frac{\sqrt{2}}{2}
    \end{bmatrix} \]
    e)
    \includegraphics[width=200px]{coord2.PNG}


    \section{Problem}
    a) It corresponds to the total amount of ingredients in the food assortment. \newline
    b)
    \[ NMX = \begin{bmatrix}
                 0.1  & 0 & 0.13 & 0\\
                 0.76 & 1 & 0.01 & 0\\
                 0.01 & 0 & 0.1  & 82
    \end{bmatrix}  \begin{bmatrix}
                                    22x_1 + 40x_2 + 50x_3\\
                                    18x_1 + 10x_2 + 3 x_3\\
                                    5 x_1 + 14x_2 + 5 x_3\\
                                    10x_1 + 10x_2 + 22x_3\\
    \end{bmatrix} \]
    c)
    \[ Y=NMX= \begin{bmatrix}
                     2.85x_1   + 5.82x_2  + 5.65x_3\\
                     34.77x_1  + 40.54x_2 + 41.05x_3\\
                     820.72x_1 + 821.8x_2 + 1805x_3
    \end{bmatrix}  \]
    \[ A^{-1} = \begin{bmatrix}
               2.85   & 5.82  & 5.65\\
               34.77  & 40.54 & 41.05\\
               820.72 & 821.8 & 1805
    \end{bmatrix} \]
    \[ X=AY\]
    \[ A = \begin{bmatrix}
               -0.47 &  0.07  & -0.0001\\
               0.35  & -0.006 & -0.01\\
               0.06  & -0.29  &  0.001
    \end{bmatrix}\]
    d)
    \[ X = \begin{bmatrix}
        x_1\\
        x_2\\
        x_3
    \end{bmatrix} = A \begin{bmatrix}
                                 50\\
                                 300\\
                                 65
    \end{bmatrix} \]
    \[ X = \begin{bmatrix}
               -2.5\\
               15\\
               -84
    \end{bmatrix}\]




\end{document}